Compiler.thy
@@ -82,15 +82,14 @@ proof -
   then obtain \<Sigma>\<^sub>u' where 
     "iter (\<tturnstile> ?cd \<leadsto>\<^sub>u) (US nmem 0 nmem 0 nmem 0 (nmem(0 := 0)) 1 (length ?cd)) \<Sigma>\<^sub>u' \<and> 
       FS (flatten_values h\<^sub>c\<^sub>e) (flatten_environment env\<^sub>h) [3 * v\<^sub>h] [] = restructure \<Sigma>\<^sub>u'" by blast
-  moreover then obtain h\<^sub>u hp\<^sub>u e\<^sub>u ep\<^sub>u vs\<^sub>u vp\<^sub>u sh\<^sub>u sp\<^sub>u where VU:
-    "\<Sigma>\<^sub>u' = US h\<^sub>u hp\<^sub>u e\<^sub>u ep\<^sub>u vs\<^sub>u vp\<^sub>u sh\<^sub>u sp\<^sub>u 0 \<and> flatten_values h\<^sub>c\<^sub>e = H h\<^sub>u hp\<^sub>u \<and> 
+  moreover then obtain h\<^sub>u hp\<^sub>u e\<^sub>u ep\<^sub>u vs\<^sub>u vp\<^sub>u where VU:
+    "\<Sigma>\<^sub>u' = USF h\<^sub>u hp\<^sub>u e\<^sub>u ep\<^sub>u vs\<^sub>u vp\<^sub>u \<and> flatten_values h\<^sub>c\<^sub>e = H h\<^sub>u hp\<^sub>u \<and> 
       flatten_environment env\<^sub>h = H e\<^sub>u ep\<^sub>u \<and> listify' vs\<^sub>u vp\<^sub>u = 3 * v\<^sub>h # []" by auto
   moreover hence VSU: "vs\<^sub>u 0 = 3 * v\<^sub>h \<and> vp\<^sub>u = 1" by auto
   ultimately have "iter (\<tturnstile> ?cd \<leadsto>\<^sub>u) (US nmem 0 nmem 0 nmem 0 (nmem(0 := 0)) 1 (length ?cd)) 
-    (US h\<^sub>u hp\<^sub>u e\<^sub>u ep\<^sub>u vs\<^sub>u 1 sh\<^sub>u sp\<^sub>u 0)" by simp
-  moreover hence "sp\<^sub>u = 0" by (metis evalu_clears_regs)
-  ultimately have EU: "iter (\<tturnstile> ?cd \<leadsto>\<^sub>u) (US nmem 0 nmem 0 nmem 0 (nmem(0 := 0)) 1 (length ?cd)) 
-    (US h\<^sub>u hp\<^sub>u e\<^sub>u ep\<^sub>u vs\<^sub>u 1 sh\<^sub>u 0 0)" by simp
+    (USF h\<^sub>u hp\<^sub>u e\<^sub>u ep\<^sub>u vs\<^sub>u 1)" by simp
+  hence EU: "iter (\<tturnstile> ?cd \<leadsto>\<^sub>u) (US nmem 0 nmem 0 nmem 0 (nmem(0 := 0)) 1 (length ?cd)) 
+    (USF h\<^sub>u hp\<^sub>u e\<^sub>u ep\<^sub>u vs\<^sub>u 1)" by simp
   let ?mem = "(\<lambda>m. case m of Hp \<Rightarrow> h\<^sub>u | Env \<Rightarrow> e\<^sub>u | Val \<Rightarrow> vs\<^sub>u | Stk \<Rightarrow> sh\<^sub>u)"
   let ?rs = "(\<lambda>r. case r of HP \<Rightarrow> hp\<^sub>u | EP \<Rightarrow> ep\<^sub>u | VP \<Rightarrow> Suc 0 | SP \<Rightarrow> 0 | ACC \<Rightarrow> 0 | ACC2 \<Rightarrow> 0)"
   let ?cd' = "(fst \<circ> assemble) ?cd"
